pancake/loop_callScript.sml
@@ -4,7 +4,7 @@
 open preamble loopLangTheory
 
 val _ = new_theory "loop_call"
-
+(*
 Definition last_def:
   (last [] = 0:num) /\
   (last xs = EL (LENGTH xs - 1) xs)
@@ -14,17 +14,52 @@ Definition butlast_def:
   (butlast [] = []) /\
   (butlast xs = TAKE (LENGTH xs - 1) xs)
 End
-
+*)
 
 Definition comp_def:
   (comp l (Call ret NONE args handler) =
    if args = [] then loopLang$Skip
    else
-   case lookup (last args) l of
+   case lookup (LAST args) l of
     | NONE => (Call ret NONE args handler)
-    | SOME n => (Call ret (SOME n) (butlast args) handler)) /\
+    | SOME n => (Call ret (SOME n) (BUTLAST args) handler)) /\
   (comp l p = p)
 End
 
+
+Definition comp_def:
+  (comp l Skip = (Skip, l)) /\
+  (comp l (Call ret NONE args handler) =
+    if args = [] then (Skip, l)
+    else
+    case lookup (LAST args) l of
+     | NONE => (Call ret NONE args handler, l)
+     | SOME n => (Call ret (SOME n) (BUTLAST args) handler, l)) /\
+  (comp l (LocValue n m) = (LocValue n m, insert n m l)) /\
+  (comp l (Assign n e) = (Assign n e,
+                          if lookup n l = NONE then l
+                          else delete n l)) /\
+  (comp l (LoadByte m n) = (LoadByte m n,
+                            case lookup n l of
+                             | NONE => l
+                             | _ => delete n l)) /\
+  (comp l (Seq p q) =
+    let (np, nl) = comp l p;
+        (nq, nl) = comp nl q in
+     (Seq np nq, nl)) /\
+  (comp l (If c n ri p q ns) =
+    let (np, nl) = comp l p;
+        (nq, ml) = comp l q in
+     (If c n ri np nq ns, LN)) /\
+  (comp l (Loop ns p ms) =
+    let (np, nl) = comp l p in
+     (Loop ns np ms, nl)) /\
+  (comp l (Mark p) =
+    let (np, nl) = comp l p in
+     (Mark np, nl)) /\
+  (comp l (FFI str n m n' m' nl) =
+     (FFI str n m n' m' nl, LN)) /\
+  (comp l p = (p, l))
+End
 
 val _ = export_theory();
