pancake/proofs/loop_callProofScript.sml
@@ -8,7 +8,314 @@ open preamble
 
 val _ = new_theory "loop_callProof";
 
+val goal =
+  “λ(prog, s). ∀res s1 l p nl.
+    evaluate (prog,s) = (res,s1) ∧ res ≠ SOME Error ∧
+    comp l prog = (p, nl) /\
+    (∀n x. lookup n l = SOME x ==> lookup n s.locals = SOME (Loc x 0)) ==>
+    evaluate (p,s) = (res,s1) /\
+    case res of
+     | NONE => (∀n x. lookup n nl = SOME x ==> lookup n s1.locals = SOME (Loc x 0))
+     | _ => T ”
 
+local
+  val ind_thm = loopSemTheory.evaluate_ind |> ISPEC goal
+    |> CONV_RULE (DEPTH_CONV PairRules.PBETA_CONV) |> REWRITE_RULE [];
+  fun list_dest_conj tm = if not (is_conj tm) then [tm] else let
+    val (c1,c2) = dest_conj tm in list_dest_conj c1 @ list_dest_conj c2 end
+  val ind_goals = ind_thm |> concl |> dest_imp |> fst |> list_dest_conj
+in
+  fun get_goal s = first (can (find_term (can (match_term (Term [QUOTE s]))))) ind_goals
+  fun compile_correct_tm () = ind_thm |> concl |> rand
+  fun the_ind_thm () = ind_thm
+end
+
+
+Theorem compile_Seq:
+  ^(get_goal "comp _ (loopLang$Seq _ _)")
+Proof
+  rpt gen_tac >>
+  strip_tac >>
+  rpt gen_tac >>
+  strip_tac >>
+  fs [loopSemTheory.evaluate_def] >>
+  pairarg_tac >> fs [comp_def] >>
+  rpt (pairarg_tac >> fs []) >>
+  fs [evaluate_def] >>
+  rpt (pairarg_tac >> fs []) >>
+  rveq >> fs [] >>
+  cases_on ‘res' = NONE’ >>
+  fs [] >> rveq >> fs []
+  >- (
+  first_x_assum (qspecl_then [‘l’, ‘np’, ‘nl'’] mp_tac) >>
+  impl_tac
+  >- (
+   fs [] >>
+   rveq >> fs [] >>
+   CCONTR_TAC >> fs []) >>
+  strip_tac >> rveq >>
+  fs [evaluate_def] >> rveq >> fs [] >>
+  last_x_assum (qspecl_then [‘nl'’, ‘nq’, ‘nl’] mp_tac) >>
+  fs []) >>
+  first_x_assum (qspecl_then [‘l’, ‘np’, ‘nl'’] mp_tac) >>
+  fs [] >>
+  strip_tac >>
+  fs [evaluate_def] >> rveq >> fs [] >>
+  cases_on ‘res’ >> fs []
+QED
+
+
+Theorem compile_LocValue:
+  ^(get_goal "comp _ (loopLang$LocValue _ _)")
+Proof
+  rpt gen_tac >>
+  strip_tac >>
+  fs [evaluate_def, comp_def] >>
+  rveq >> fs [] >>
+  fs [evaluate_def] >>
+  cases_on ‘res’ >> fs []  >>
+  every_case_tac >> fs [] >>
+  last_x_assum (assume_tac o GSYM) >>
+  rveq >> fs [set_var_def] >>
+  rw [] >>
+  fs [lookup_insert] >>
+  every_case_tac >> fs []
+QED
+
+Theorem compile_Assign:
+  ^(get_goal "comp _ (loopLang$Assign _ _)")
+Proof
+  rpt gen_tac >>
+  strip_tac >>
+  fs [evaluate_def, comp_def] >>
+  rveq >> fs [] >>
+  fs [evaluate_def] >>
+  cases_on ‘res’ >> fs []  >>
+  every_case_tac >> fs [] >>
+  last_x_assum (assume_tac o GSYM) >>
+  rveq >> fs [set_var_def] >>
+  rw [] >>
+  fs [lookup_insert] >>
+  every_case_tac >> fs [] >>
+  rveq >> fs [lookup_delete]
+QED
+
+Theorem compile_LoadByte:
+  ^(get_goal "comp _ (loopLang$LoadByte _ _)")
+Proof
+  rpt gen_tac >>
+  strip_tac >>
+  fs [evaluate_def, comp_def] >>
+  rveq >> fs [] >>
+  fs [evaluate_def] >>
+  cases_on ‘res’ >> fs []  >>
+  every_case_tac >> fs [] >>
+  last_x_assum (assume_tac o GSYM) >>
+  rveq >> fs [set_var_def] >>
+  rw [] >>
+  fs [lookup_insert] >>
+  every_case_tac >> fs [] >>
+  rveq >> fs [lookup_delete]
+QED
+
+
+Theorem compile_Mark:
+  ^(get_goal "comp _ (loopLang$Mark _)")
+Proof
+  rpt gen_tac >>
+  strip_tac >>
+  rpt gen_tac >>
+  fs [comp_def] >>
+  pairarg_tac >> fs [] >> rveq >>
+  fs [] >>
+  strip_tac >> fs [] >>
+  rveq >> fs [] >>
+  fs [evaluate_def] >>
+  res_tac >> fs []
+QED
+
+
+Theorem compile_FFI:
+  ^(get_goal "comp _ (loopLang$FFI _ _ _ _ _ _)")
+Proof
+  rpt gen_tac >>
+  strip_tac >>
+  rpt gen_tac >>
+  fs [comp_def] >>
+  every_case_tac >> fs [] >>
+  rveq >> fs [] >>
+  fs [evaluate_def] >>
+  every_case_tac >> fs [] >> rveq >>
+  fs [] >>
+  fs [cut_state_def] >> rveq >> fs [lookup_def]
+QED
+
+
+Theorem compile_If:
+  ^(get_goal "comp _ (loopLang$If _ _ _ _ _ _)")
+Proof
+  rpt gen_tac >>
+  strip_tac >>
+  rpt gen_tac >>
+  strip_tac >>
+  fs [evaluate_def, comp_def] >>
+  rveq >> fs [] >>
+  fs [evaluate_def, CaseEq "option", CaseEq "word_loc"] >>
+  rveq >> fs [] >>
+  cases_on ‘word_cmp cmp x y’ >> fs [] >> rveq >>
+  pairarg_tac >> fs [] >>
+  pairarg_tac >> fs [] >> rveq >> fs []
+  >- (
+   cases_on ‘evaluate (c1,s)’ >> fs [] >>
+   fs [cut_res_def] >>
+   cases_on ‘q ≠ NONE’ >> fs [] >> rveq >> fs []
+   >- (
+    last_x_assum drule >>
+    fs [] >>
+    strip_tac >> fs [] >>
+    fs [evaluate_def] >>
+    cases_on ‘q’ >> fs [cut_res_def]) >>
+   last_x_assum drule >>
+   fs [] >>
+   strip_tac >> fs [CaseEq "option"] >>
+   rveq >> fs []  >>
+   fs [evaluate_def] >>
+   fs [cut_res_def] >>
+   cases_on ‘v.clock = 0’ >> fs [] >> rveq >> fs [] >>
+   fs [dec_clock_def, lookup_inter, cut_state_def] >>
+   qpat_x_assum ‘r with locals := _ = _’ (assume_tac o GSYM) >>
+   rveq >> fs [] >>
+   rw [] >>
+   fs [CaseEq "option"] >> rveq >> fs [lookup_inter] >>
+   res_tac >>
+   TOP_CASE_TAC >> fs [] >> rveq >>
+   fs [lookup_def] >>
+   TOP_CASE_TAC >> fs []) >>
+  cases_on ‘evaluate (c2,s)’ >> fs [] >>
+  fs [cut_res_def] >>
+  cases_on ‘q ≠ NONE’ >> fs [] >> rveq >> fs []
+  >- (
+   last_x_assum drule >>
+   fs [] >>
+   strip_tac >> fs [] >>
+   fs [evaluate_def] >>
+   cases_on ‘q’ >> fs [cut_res_def]) >>
+  last_x_assum drule >>
+  fs [] >>
+  strip_tac >> fs [CaseEq "option"] >>
+  rveq >> fs []  >>
+  fs [evaluate_def] >>
+  fs [cut_res_def] >>
+  cases_on ‘v.clock = 0’ >> fs [] >> rveq >> fs [] >>
+  fs [dec_clock_def, lookup_inter, cut_state_def] >>
+  qpat_x_assum ‘r with locals := _ = _’ (assume_tac o GSYM) >>
+  rveq >> fs [] >>
+  rw [] >>
+  fs [CaseEq "option"] >> rveq >> fs [lookup_inter] >>
+  res_tac >>
+  TOP_CASE_TAC >> fs [] >> rveq >>
+  fs [lookup_def] >>
+  TOP_CASE_TAC >> fs []
+QED
+
+Theorem compile_StoreByte:
+  ^(get_goal "comp _ (loopLang$StoreByte _ _)")
+Proof
+  rpt gen_tac >>
+  strip_tac >>
+  fs [evaluate_def, comp_def] >>
+  rveq >> fs [] >>
+  fs [evaluate_def] >>
+  cases_on ‘res’ >> fs []  >>
+  every_case_tac >> fs [] >>
+  last_x_assum (assume_tac o GSYM) >>
+  rveq >> fs []
+QED
+
+
+Theorem compile_Store:
+  ^(get_goal "comp _ (loopLang$Store _ _)")
+Proof
+  rpt gen_tac >>
+  strip_tac >>
+  fs [evaluate_def, comp_def] >>
+  rveq >> fs [] >>
+  fs [evaluate_def] >>
+  cases_on ‘res’ >> fs []  >>
+  every_case_tac >> fs [mem_store_def] >>
+  last_x_assum (assume_tac o GSYM) >>
+  rveq >> fs []
+QED
+
+
+Theorem compile_Call:
+  ^(get_goal "comp _ (loopLang$Call _ _ _ _)")
+Proof
+  cheat
+QED
+
+Theorem compile_Loop:
+  ^(get_goal "comp _ (loopLang$Loop _ _ _)")
+Proof
+  rpt gen_tac >>
+  strip_tac >>
+  rpt gen_tac >>
+  strip_tac >>
+  fs [Once evaluate_def, comp_def] >>
+  cases_on ‘cut_res live_in (NONE:'a result option,s)’ >> fs [] >>
+  rveq >> fs [] >>
+  pairarg_tac >>
+  fs [] >>
+  reverse (cases_on ‘q’) >> fs [] >> rveq >> fs []
+  >- fs [Once evaluate_def] >>
+  cases_on ‘evaluate (body,r)’ >> fs [] >>
+  cases_on ‘q’ >> fs [] >>
+  cases_on ‘x’ >> fs [] >>
+  rveq >> fs [] >>
+  fs [Once evaluate_def] >>
+  res_tac >> fs [] >>
+  cheat
+QED
+
+
+Theorem compile_others:
+  ^(get_goal "comp _ loopLang$Skip") ∧
+  ^(get_goal "comp _ loopLang$Fail") ∧
+  ^(get_goal "comp _ loopLang$Tick") ∧
+  ^(get_goal "comp _ loopLang$Break") ∧
+  ^(get_goal "comp _ loopLang$Continue") ∧
+  ^(get_goal "comp _ (loopLang$Raise _)") ∧
+  ^(get_goal "comp _ (loopLang$Return _)") ∧
+  ^(get_goal "comp _ (loopLang$SetGlobal _ _)")
+Proof
+  rw [] >>
+  fs [evaluate_def, comp_def] >>
+  rveq >> fs [] >>
+  fs [evaluate_def] >>
+  cases_on ‘res’ >>
+  fs [] >>
+  every_case_tac >> fs [dec_clock_def] >>
+  last_x_assum (assume_tac o GSYM) >>
+  rveq >> fs [set_globals_def]
+QED
+
+
+Theorem compile_correct:
+  ^(compile_correct_tm())
+Proof
+  match_mp_tac (the_ind_thm()) >>
+  EVERY (map strip_assume_tac
+         [compile_others,compile_LocValue,compile_LoadByte,compile_StoreByte,
+          compile_Mark, compile_Assign, compile_Store,
+          compile_Call, compile_Seq, compile_If, compile_FFI, compile_Loop]) >>
+  asm_rewrite_tac [] >> rw [] >> rpt (pop_assum kall_tac)
+QED
+
+
+
+
+(*
+(*
 Theorem butlast_cons:
   !xs x. xs <> [] ==>
     butlast (x::xs) = x::butlast xs
@@ -105,17 +412,105 @@ Proof
   fs [get_vars_def] >>
   every_case_tac >> fs []
 QED
-
+*)
 
 Theorem comp_correct:
-  loopSem$evaluate (prog,s) = (res,s1) ∧
+  !prog s res s1 l. loopSem$evaluate (prog,s) = (res,s1) ∧
   res ≠ SOME Error ∧
-  (∀n x. lookup n l = SOME x ==> lookup n s.locals = SOME (Loc x 0)) ⇒
-  evaluate (comp l prog,s) = (res,s1)
+  (∀n x. lookup n l = SOME x ==> lookup n s.locals = SOME (Loc x 0)) /\
+  comp l prog = (np, nl) /\ evaluate (np,s) = (res',s1') ==>
+   (res = res' /\ s1 = s1' /\
+    (∀n x. lookup n nl = SOME x ==> lookup n s1.locals = SOME (Loc x 0)))
 Proof
-  rw [] >>
+  ho_match_mp_tac loopSemTheory.evaluate_ind >>
+
+
+
   cases_on ‘prog’ >>
-  fs [loop_callTheory.comp_def] >>
+  fs [loop_callTheory.comp_def]
+  >- (fs [evaluate_def] >> rveq >> fs [])
+  >- (
+   fs [evaluate_def] >>
+   every_case_tac >> fs [] >> rveq  >> fs [] >>
+   rw []
+   >- (
+    fs [set_var_def] >>
+    fs [lookup_insert] >>
+    TOP_CASE_TAC >> fs []) >>
+   fs [set_var_def] >>
+   fs [lookup_insert] >>
+   TOP_CASE_TAC >> fs [] >> rveq >>
+   fs [lookup_delete])
+  >- (
+   fs [evaluate_def] >>
+   every_case_tac >> fs [] >> rveq  >> fs [] >>
+   rw [] >>
+   fs [mem_store_def] >>
+   pop_assum mp_tac >>
+   pop_assum (assume_tac o GSYM) >>
+   fs [])
+  >- (
+   fs [evaluate_def] >>
+   every_case_tac >> fs [] >> rveq  >> fs [] >>
+   rw [] >>
+   fs [set_globals_def])
+  >- (
+   fs [evaluate_def] >>
+   every_case_tac >> fs [] >> rveq  >> fs [] >>
+   rw [] >>
+   fs [set_var_def, lookup_insert] >>
+   TOP_CASE_TAC >> fs [] >>
+   rveq >> fs [lookup_delete])
+  >- (
+   fs [evaluate_def] >>
+   every_case_tac >> fs [] >> rveq  >> fs [])
+
+
+
+  >- (
+   fs [evaluate_def] >>
+   pairarg_tac >> fs [] >>
+   rveq >> fs [] >>
+   cases_on ‘res' = NONE’ >> fs [] >>
+   rveq >> fs []
+
+
+   pairarg_tac >> fs [] >>
+   pairarg_tac >> fs [] >>
+   pairarg_tac >> fs [] >> rveq >>
+   every_case_tac >> fs [] >> rveq  >> fs [] >>
+   pairarg_tac >> fs [] >> rveq >>
+   pairarg_tac >> fs [] >> rveq >>
+   every_case_tac >> fs [] >>
+
+
+   )
+
+   )
+
+
+
+
+   )
+
+
+
+
+
+
+   )
+
+
+
+   )
+
+    )
+
+      rveq >> fs [])
+
+
+
+
   qmatch_goalsub_rename_tac ‘Call ret dest args hdl’ >>
   cases_on ‘dest’ >>
   fs [loop_callTheory.comp_def] >>
@@ -152,6 +547,6 @@ Proof
   TOP_CASE_TAC >> fs [] >>
   fs [LENGTH_FRONT]
 QED
-
+*)
 
 val _ = export_theory();
